@prefix : <https://greeninfratwins.com/ns/grit#> .
@prefix owl: <http://www.w3.org/2002/07/owl#> .
@prefix rdf: <http://www.w3.org/1999/02/22-rdf-syntax-ns#> .
@prefix xml: <http://www.w3.org/XML/1998/namespace> .
@prefix xsd: <http://www.w3.org/2001/XMLSchema#> .
@prefix rdfs: <http://www.w3.org/2000/01/rdf-schema#> .
@base <https://greeninfratwins.com/ns/grit#> .

<https://greeninfratwins.com/ns/grit#> rdf:type owl:Ontology ;
                                        <http://purl.org/dc/terms/contributor> _:genid1 ,
                                                                               _:genid3 ;
                                        <http://purl.org/dc/terms/created> "2024-08-01"^^xsd:date ;
                                        <http://purl.org/dc/terms/creator> _:genid5 ;
                                        <http://purl.org/dc/terms/description> "The GreenInfraTwins (GRIT) Ontology is used for establishing digital twins for the sustainability assessment of transportaion infrastructure in Germany, Austria, and Switzerland. The aim of the research project is to conceptualise and demonstrate sustainability-related decision support through the use of digital twins of engineering structures. To this end, digital twins of engineering structures are created, enriched with data and used to calculate key indicators for sustainability analyses. "@en ;
                                        <http://purl.org/dc/terms/license> <https://creativecommons.org/licenses/by/4.0/> ;
                                        <http://purl.org/dc/terms/modified> "2025-04-29"^^xsd:date ;
                                        <http://purl.org/dc/terms/rights> "Copyright 2024 by Chair of Computing in Engineering, Ruhr University Bochum" ;
                                        <http://purl.org/dc/terms/source> "https://www.greeninfratwins.com" ;
                                        <http://purl.org/dc/terms/title> "GreenInfraTwins (GRIT) Ontology"@en ;
                                        <http://purl.org/vocab/vann/preferredNamespacePrefix> "grit" ;
                                        <http://purl.org/vocab/vann/preferredNamespaceUri> <https://greeninfratwins.com/ns/grit#> ;
                                        owl:versionInfo "1.0" .

_:genid1 rdf:type <https://schema.org/Person> ;
          <https://schema.org/email> <mailto:liu.liu-m6r@rub.de> ;
          <https://schema.org/identifier> <https://orcid.org/0000-0001-5907-7609> ;
          <https://schema.org/memberOf> _:genid2 ;
          <https://schema.org/name> "Liu Liu" .

_:genid3 rdf:type <https://schema.org/Person> ;
          <https://schema.org/email> <mailto:simon.kosse@rub.de> ;
          <https://schema.org/identifier> <https://orcid.org/0000-0002-6391-784X> ;
          <https://schema.org/memberOf> _:genid4 ;
          <https://schema.org/name> "Simon Kosse" .

_:genid5 rdf:type <https://schema.org/Person> ;
          <https://schema.org/email> <mailto:philipp.hagedorn-n6v@rub.de> ;
          <https://schema.org/identifier> <https://orcid.org/0000-0002-6249-243X> ;
          <https://schema.org/memberOf> _:genid6 ;
          <https://schema.org/name> "Philipp Hagedorn" .

_:genid2 <https://schema.org/identifier> <https://www.inf.bi.ruhr-uni-bochum.de/iib/lehrstuhl/mitarbeiter/liu_liu.html.en> ;
          <https://schema.org/name> "Ruhr University Bochum" .

_:genid4 <https://schema.org/identifier> <https://www.inf.bi.ruhr-uni-bochum.de/iib/lehrstuhl/mitarbeiter/simon_kosse.html.en> ;
          <https://schema.org/name> "Ruhr University Bochum" .

_:genid6 <https://schema.org/identifier> <https://www.inf.bi.ruhr-uni-bochum.de/iib/lehrstuhl/mitarbeiter/philipp_hagedorn.html.en> ;
          <https://schema.org/name> "Ruhr University Bochum" .

#################################################################
#    Annotation properties
#################################################################

###  http://purl.org/dc/terms/contributor
<http://purl.org/dc/terms/contributor> rdf:type owl:AnnotationProperty .


###  http://purl.org/dc/terms/created
<http://purl.org/dc/terms/created> rdf:type owl:AnnotationProperty .


###  http://purl.org/dc/terms/creator
<http://purl.org/dc/terms/creator> rdf:type owl:AnnotationProperty .


###  http://purl.org/dc/terms/description
<http://purl.org/dc/terms/description> rdf:type owl:AnnotationProperty .


###  http://purl.org/dc/terms/license
<http://purl.org/dc/terms/license> rdf:type owl:AnnotationProperty .


###  http://purl.org/dc/terms/modified
<http://purl.org/dc/terms/modified> rdf:type owl:AnnotationProperty .


###  http://purl.org/dc/terms/rights
<http://purl.org/dc/terms/rights> rdf:type owl:AnnotationProperty .


###  http://purl.org/dc/terms/source
<http://purl.org/dc/terms/source> rdf:type owl:AnnotationProperty .


###  http://purl.org/dc/terms/title
<http://purl.org/dc/terms/title> rdf:type owl:AnnotationProperty .


###  http://purl.org/vocab/vann/preferredNamespacePrefix
<http://purl.org/vocab/vann/preferredNamespacePrefix> rdf:type owl:AnnotationProperty .


###  http://purl.org/vocab/vann/preferredNamespaceUri
<http://purl.org/vocab/vann/preferredNamespaceUri> rdf:type owl:AnnotationProperty .


###  https://greeninfratwins.com/ns/grit#belongsToPredefinedSetOfIndicators
:belongsToPredefinedSetOfIndicators rdf:type owl:AnnotationProperty .


###  https://schema.org/email
<https://schema.org/email> rdf:type owl:AnnotationProperty .


###  https://schema.org/identifier
<https://schema.org/identifier> rdf:type owl:AnnotationProperty .


###  https://schema.org/memberOf
<https://schema.org/memberOf> rdf:type owl:AnnotationProperty .


###  https://schema.org/name
<https://schema.org/name> rdf:type owl:AnnotationProperty .


#################################################################
#    Datatypes
#################################################################

###  http://www.w3.org/2001/XMLSchema#date
xsd:date rdf:type rdfs:Datatype .


#################################################################
#    Object Properties
#################################################################

###  https://greeninfratwins.com/ns/grit#afterActivity
:afterActivity rdf:type owl:ObjectProperty ;
               rdfs:subPropertyOf owl:topObjectProperty ;
               rdfs:domain :Activity ;
               rdfs:range :Activity ;
               rdfs:comment "Establishes a procedural order of activities." ;
               rdfs:label "after activity" .


###  https://greeninfratwins.com/ns/grit#connectedServices
:connectedServices rdf:type owl:ObjectProperty ;
                   rdfs:subPropertyOf owl:topObjectProperty ;
                   rdfs:domain :GreenInfraTwin ;
                   rdfs:comment "The services connected to a DT, e.g., ICDD container." ;
                   rdfs:label "connected services" .


###  https://greeninfratwins.com/ns/grit#frequencyPerYear
:frequencyPerYear rdf:type owl:ObjectProperty ;
                  rdfs:subPropertyOf owl:topObjectProperty ;
                  rdfs:domain :Measure ;
                  rdfs:comment "Displays the frequency of a measure per year." ;
                  rdfs:label "frequency per year" .


###  https://greeninfratwins.com/ns/grit#hasAsessment
:hasAsessment rdf:type owl:ObjectProperty ;
              rdfs:subPropertyOf owl:topObjectProperty ;
              rdfs:domain :GreenInfraTwin ;
              rdfs:range :Assessment ;
              rdfs:comment "The connection beween the DT and the use case / asessment." ;
              rdfs:label "has asessment" .


###  https://greeninfratwins.com/ns/grit#hasExternalCalculationApplication
:hasExternalCalculationApplication rdf:type owl:ObjectProperty ;
                                   rdfs:subPropertyOf owl:topObjectProperty ;
                                   rdfs:domain :ComplexComputedValueIndicator ;
                                   rdfs:comment "Indicates the external application in which the calculation of an indicator is performed." ;
                                   rdfs:label "has external calculation application" .


###  https://greeninfratwins.com/ns/grit#hasExternalCalculationServiceUrl
:hasExternalCalculationServiceUrl rdf:type owl:ObjectProperty ;
                                  rdfs:subPropertyOf owl:topObjectProperty ;
                                  rdfs:domain :SimpleComputedValueIndicator ;
                                  rdfs:comment "The URL of a calculation service that can calculate the indicator based on the given formula and the respective variables." ;
                                  rdfs:label "has calculation service" .


###  https://greeninfratwins.com/ns/grit#hasFormula
:hasFormula rdf:type owl:ObjectProperty ;
            rdfs:subPropertyOf owl:topObjectProperty ;
            rdfs:domain :SimpleComputedValueIndicator ;
            rdfs:comment "The calculation formular of a simple computed value indicator." ;
            rdfs:label "has formula" .


###  https://greeninfratwins.com/ns/grit#hasIndicator
:hasIndicator rdf:type owl:ObjectProperty ;
              rdfs:subPropertyOf owl:topObjectProperty ;
              rdfs:domain :IndicatorSet ;
              rdfs:range :Indicator ;
              rdfs:comment "The connection between an indicator set and the indicator. This relation may occur multiple times." ;
              rdfs:label "has indicator" .


###  https://greeninfratwins.com/ns/grit#hasIndicatorSet
:hasIndicatorSet rdf:type owl:ObjectProperty ;
                 rdfs:subPropertyOf owl:topObjectProperty ;
                 rdfs:domain :Activity ;
                 rdfs:range :IndicatorSet ;
                 rdfs:comment "Establishes the connection between the activity and the respective indicators." ;
                 rdfs:label "has indicator set" .


###  https://greeninfratwins.com/ns/grit#hasIndicatorType
:hasIndicatorType rdf:type owl:ObjectProperty ;
                  rdfs:subPropertyOf owl:topObjectProperty ;
                  rdfs:domain :Indicator ;
                  rdfs:range :IndicatorType ;
                  rdfs:comment "Provides the indicator type." ;
                  rdfs:label "has indicator type" .


###  https://greeninfratwins.com/ns/grit#hasKey
:hasKey rdf:type owl:ObjectProperty ;
        rdfs:subPropertyOf owl:topObjectProperty ;
        rdfs:domain :IndicatorVariable ;
        owl:propertyDisjointWith :hasValue ;
        rdfs:comment "The key of a variable exactly as it appears in the calculation formula, e.g. v (for volume)." ;
        rdfs:label "has key" .


###  https://greeninfratwins.com/ns/grit#hasMeasure
:hasMeasure rdf:type owl:ObjectProperty ;
            rdfs:subPropertyOf owl:topObjectProperty ;
            rdfs:domain :Assessment ;
            rdfs:range :Measure ;
            rdfs:comment "The measures that are part of one assessment / use case." ;
            rdfs:label "has measure" .


###  https://greeninfratwins.com/ns/grit#hasMeasureVariant
:hasMeasureVariant rdf:type owl:ObjectProperty ;
                   rdfs:subPropertyOf owl:topObjectProperty ;
                   rdfs:domain :Measure ;
                   rdfs:range :MeasureVariant ;
                   rdfs:comment "A measure variant can be used to compare multiple variants of the same measure during the assessment." ;
                   rdfs:label "has measure variant" .


###  https://greeninfratwins.com/ns/grit#hasUnit
:hasUnit rdf:type owl:ObjectProperty ;
         rdfs:subPropertyOf owl:topObjectProperty ;
         rdfs:domain :IndicatorVariable ;
         rdfs:range <https://qudt.org/schema/qudt/Unit> ;
         rdfs:comment "The unit that a value refers to." ;
         rdfs:label "has unit" .


###  https://greeninfratwins.com/ns/grit#hasValue
:hasValue rdf:type owl:ObjectProperty ;
          rdfs:subPropertyOf owl:topObjectProperty ;
          rdfs:domain :IndicatorVariable ;
          rdfs:comment "The value that should be computed by a calculation service for a given variable." ;
          rdfs:label "has value" .


###  https://greeninfratwins.com/ns/grit#hasVariable
:hasVariable rdf:type owl:ObjectProperty ;
             rdfs:subPropertyOf owl:topObjectProperty ;
             rdfs:domain :SimpleComputedValueIndicator ;
             rdfs:range :IndicatorVariable ;
             rdfs:comment "The connection between the indicator ant the variables of an indicator." ;
             rdfs:label "has variable" .


###  https://greeninfratwins.com/ns/grit#involvesActivities
:involvesActivities rdf:type owl:ObjectProperty ;
                    rdfs:subPropertyOf owl:topObjectProperty ;
                    rdfs:domain :Measure ,
                                :MeasureVariant ;
                    rdfs:range :Activity ;
                    rdfs:comment "The activities that are performed within a measure or a measure variant." ;
                    rdfs:label "involves activities" .


###  https://greeninfratwins.com/ns/grit#isDefinedBy
:isDefinedBy rdf:type owl:ObjectProperty ;
             rdfs:subPropertyOf owl:topObjectProperty ;
             rdfs:domain :Assessment ;
             rdfs:range :SpecifiedUseCase ;
             rdfs:label "has specified use case" .


###  https://greeninfratwins.com/ns/grit#mapsToLbdProperty
:mapsToLbdProperty rdf:type owl:ObjectProperty ;
                   rdfs:subPropertyOf owl:topObjectProperty ;
                   rdfs:domain :IndicatorVariable ;
                   rdfs:range rdfs:Resource ;
                   rdfs:comment "This property is used to map a variable of an indicator to a property present in the RDF dataset of the digital twin." ;
                   rdfs:label "maps to lbd property" .


###  https://greeninfratwins.com/ns/grit#grit:belongsToPredefinedSetOfIndicators
:grit:belongsToPredefinedSetOfIndicators rdf:type owl:ObjectProperty ;
                                         rdfs:subPropertyOf owl:topObjectProperty ;
                                         rdfs:domain :IndicatorType ;
                                         rdfs:range :IndicatorSet ;
                                         rdfs:label "belongs to predefined set of indicators" .


#################################################################
#    Data properties
#################################################################

###  https://greeninfratwins.com/ns/grit#hasIcddContainerID
:hasIcddContainerID rdf:type owl:DatatypeProperty ;
                    rdfs:subPropertyOf owl:topDataProperty ;
                    rdfs:domain :GreenInfraTwin ;
                    rdfs:range xsd:anyURI ;
                    rdfs:label "has icdd container ID" .


###  https://greeninfratwins.com/ns/grit#hasIcddModelID
:hasIcddModelID rdf:type owl:DatatypeProperty ;
                rdfs:subPropertyOf owl:topDataProperty ;
                rdfs:domain :Activity ;
                rdfs:range xsd:string ;
                rdfs:label "has icdd model id" .


###  https://greeninfratwins.com/ns/grit#hasIcddProjectID
:hasIcddProjectID rdf:type owl:DatatypeProperty ;
                  rdfs:subPropertyOf owl:topDataProperty ;
                  rdfs:domain :GreenInfraTwin ;
                  rdfs:range xsd:anyURI ;
                  rdfs:label "has icdd project ID" .


###  https://greeninfratwins.com/ns/grit#hasIfcGuid
:hasIfcGuid rdf:type owl:DatatypeProperty ;
            rdfs:subPropertyOf owl:topDataProperty ;
            rdfs:domain :Activity ;
            rdfs:range xsd:string .


###  https://greeninfratwins.com/ns/grit#hasIndicatorID
:hasIndicatorID rdf:type owl:DatatypeProperty ;
                rdfs:subPropertyOf owl:topDataProperty ;
                rdfs:domain :IndicatorType ;
                rdfs:range xsd:string .


#################################################################
#    Classes
#################################################################

###  http://www.w3.org/2000/01/rdf-schema#Resource
rdfs:Resource rdf:type owl:Class .


###  http://www.w3.org/2001/XMLSchema#decimal
xsd:decimal rdf:type owl:Class .


###  http://www.w3.org/2001/XMLSchema#int
xsd:int rdf:type owl:Class .


###  https://greeninfratwins.com/ns/grit#Activity
:Activity rdf:type owl:Class ;
          rdfs:subClassOf owl:Thing ,
                          [ rdf:type owl:Restriction ;
                            owl:onProperty :afterActivity ;
                            owl:someValuesFrom :Activity
                          ] ,
                          [ rdf:type owl:Restriction ;
                            owl:onProperty :hasIfcGuid ;
                            owl:someValuesFrom xsd:string
                          ] ,
                          [ rdf:type owl:Restriction ;
                            owl:onProperty :hasIndicatorSet ;
                            owl:qualifiedCardinality "1"^^xsd:nonNegativeInteger ;
                            owl:onClass :IndicatorSet
                          ] ,
                          [ rdf:type owl:Restriction ;
                            owl:onProperty :hasIcddModelID ;
                            owl:cardinality "1"^^xsd:nonNegativeInteger
                          ] ;
          rdfs:comment "The activity that is performed in a particularly sequence within a measure or measure variant." ;
          rdfs:label "Activity" .


###  https://greeninfratwins.com/ns/grit#Assessment
:Assessment rdf:type owl:Class ;
            rdfs:subClassOf owl:Thing ,
                            [ rdf:type owl:Restriction ;
                              owl:onProperty :hasMeasure ;
                              owl:someValuesFrom :Measure
                            ] ,
                            [ rdf:type owl:Restriction ;
                              owl:onProperty :isDefinedBy ;
                              owl:maxQualifiedCardinality "1"^^xsd:nonNegativeInteger ;
                              owl:onClass :SpecifiedUseCase
                            ] ;
            rdfs:comment "The use case that is performed in a DT." ;
            rdfs:label "Assessment defined by a specified Use Case" .


###  https://greeninfratwins.com/ns/grit#ComplexComputedValueIndicator
:ComplexComputedValueIndicator rdf:type owl:Class ;
                               rdfs:subClassOf :ValueIndicator ,
                                               [ rdf:type owl:Restriction ;
                                                 owl:onProperty :hasVariable ;
                                                 owl:someValuesFrom :IndicatorVariable
                                               ] ,
                                               [ rdf:type owl:Restriction ;
                                                 owl:onProperty :hasExternalCalculationApplication ;
                                                 owl:cardinality "1"^^xsd:nonNegativeInteger
                                               ] ;
                               owl:disjointWith :ConstantValueIndicator ,
                                                :SimpleComputedValueIndicator ;
                               rdfs:comment "An indicator that cannot be calculated by just a given formula but in expert software." ;
                               rdfs:label "Complex computed value indicator" .


###  https://greeninfratwins.com/ns/grit#ConstantValueIndicator
:ConstantValueIndicator rdf:type owl:Class ;
                        rdfs:subClassOf :ValueIndicator ;
                        owl:disjointWith :SimpleComputedValueIndicator ;
                        rdfs:comment "An indicator that does not change over time." ;
                        rdfs:label "Constant value indicator" .


###  https://greeninfratwins.com/ns/grit#GreenInfraTwin
:GreenInfraTwin rdf:type owl:Class ;
                rdfs:subClassOf owl:Thing ,
                                [ rdf:type owl:Restriction ;
                                  owl:onProperty :hasAsessment ;
                                  owl:someValuesFrom :Assessment
                                ] ,
                                [ rdf:type owl:Restriction ;
                                  owl:onProperty :connectedServices ;
                                  owl:minCardinality "0"^^xsd:nonNegativeInteger
                                ] ,
                                [ rdf:type owl:Restriction ;
                                  owl:onProperty :hasIcddContainerID ;
                                  owl:qualifiedCardinality "1"^^xsd:nonNegativeInteger ;
                                  owl:onDataRange xsd:anyURI
                                ] ,
                                [ rdf:type owl:Restriction ;
                                  owl:onProperty :hasIcddProjectID ;
                                  owl:qualifiedCardinality "1"^^xsd:nonNegativeInteger ;
                                  owl:onDataRange xsd:anyURI
                                ] ;
                rdfs:comment "The instance of a DT for sustainability asessment." ;
                rdfs:label "GreenInfraTwin Demonstrator" .


###  https://greeninfratwins.com/ns/grit#Indicator
:Indicator rdf:type owl:Class ;
           rdfs:subClassOf owl:Thing ,
                           [ rdf:type owl:Restriction ;
                             owl:onProperty :hasIndicatorType ;
                             owl:qualifiedCardinality "1"^^xsd:nonNegativeInteger ;
                             owl:onClass :IndicatorType
                           ] ;
           rdfs:comment "The generic indicator class, can be subtyped regarding their caracteristics and their value calculation methods." ;
           rdfs:label "Indicator" .


###  https://greeninfratwins.com/ns/grit#IndicatorSet
:IndicatorSet rdf:type owl:Class ;
              rdfs:subClassOf owl:Thing ,
                              [ rdf:type owl:Restriction ;
                                owl:onProperty :hasIndicator ;
                                owl:someValuesFrom :Indicator
                              ] ;
              rdfs:comment "A set of indicators that is referenced by a specific activity." ;
              rdfs:label "Indicator set" .


###  https://greeninfratwins.com/ns/grit#IndicatorType
:IndicatorType rdf:type owl:Class ;
               rdfs:subClassOf owl:Thing ,
                               [ rdf:type owl:Restriction ;
                                 owl:onProperty :hasIndicatorID ;
                                 owl:qualifiedCardinality "1"^^xsd:nonNegativeInteger ;
                                 owl:onDataRange xsd:string
                               ] ;
               rdfs:comment "A type for identifying indicators that should be aggregated in the overall calculation, e.g. GWP." ;
               rdfs:label "Indicator type" .


###  https://greeninfratwins.com/ns/grit#IndicatorVariable
:IndicatorVariable rdf:type owl:Class ;
                   rdfs:subClassOf owl:Thing ,
                                   [ rdf:type owl:Restriction ;
                                     owl:onProperty :hasKey ;
                                     owl:qualifiedCardinality "1"^^xsd:nonNegativeInteger ;
                                     owl:onClass xsd:string
                                   ] ,
                                   [ rdf:type owl:Restriction ;
                                     owl:onProperty :hasUnit ;
                                     owl:qualifiedCardinality "1"^^xsd:nonNegativeInteger ;
                                     owl:onClass <https://qudt.org/schema/qudt/Unit>
                                   ] ,
                                   [ rdf:type owl:Restriction ;
                                     owl:onProperty :hasValue ;
                                     owl:qualifiedCardinality "1"^^xsd:nonNegativeInteger ;
                                     owl:onClass xsd:decimal
                                   ] ,
                                   [ rdf:type owl:Restriction ;
                                     owl:onProperty :mapsToLbdProperty ;
                                     owl:cardinality "1"^^xsd:nonNegativeInteger
                                   ] ;
                   rdfs:comment "The variable that is used to calculated for an indicator, consists of a key (the variable identified) and a value (the numerical value)" ;
                   rdfs:label "Indicator variable" .


###  https://greeninfratwins.com/ns/grit#Measure
:Measure rdf:type owl:Class ;
         rdfs:subClassOf owl:Thing ,
                         [ rdf:type owl:Restriction ;
                           owl:onProperty :hasMeasureVariant ;
                           owl:someValuesFrom :MeasureVariant
                         ] ,
                         [ rdf:type owl:Restriction ;
                           owl:onProperty :involvesActivities ;
                           owl:someValuesFrom :Activity
                         ] ,
                         [ rdf:type owl:Restriction ;
                           owl:onProperty :frequencyPerYear ;
                           owl:qualifiedCardinality "1"^^xsd:nonNegativeInteger ;
                           owl:onClass xsd:int
                         ] ;
         rdfs:comment "The definition of a measure." ;
         rdfs:label "Measure" .


###  https://greeninfratwins.com/ns/grit#MeasureIndicator
:MeasureIndicator rdf:type owl:Class ;
                  rdfs:subClassOf :Indicator ;
                  owl:disjointWith :ReliabilityIndicator ,
                                   :TechnicalQualityIndicator ;
                  rdfs:comment "An indicator used for being calculated in a measure for sustainability asessment." ;
                  rdfs:label "Measure indicator" .


###  https://greeninfratwins.com/ns/grit#MeasureVariant
:MeasureVariant rdf:type owl:Class ;
                rdfs:subClassOf owl:Thing ,
                                [ rdf:type owl:Restriction ;
                                  owl:onProperty :involvesActivities ;
                                  owl:someValuesFrom :Activity
                                ] ;
                rdfs:comment "An optional variant of the measure. A measure can either directly involve activities directly, or, if needed, can have multiple variants that each involve activities." ;
                rdfs:label "Measure variant" .


###  https://greeninfratwins.com/ns/grit#ReliabilityIndicator
:ReliabilityIndicator rdf:type owl:Class ;
                      rdfs:subClassOf :Indicator ;
                      owl:disjointWith :TechnicalQualityIndicator ;
                      rdfs:comment "An indicator depicting the reliability of a measure." ;
                      rdfs:label "Reliability indicator" .


###  https://greeninfratwins.com/ns/grit#SimpleComputedValueIndicator
:SimpleComputedValueIndicator rdf:type owl:Class ;
                              rdfs:subClassOf :ValueIndicator ,
                                              [ rdf:type owl:Restriction ;
                                                owl:onProperty :hasVariable ;
                                                owl:someValuesFrom :IndicatorVariable
                                              ] ,
                                              [ rdf:type owl:Restriction ;
                                                owl:onProperty :hasExternalCalculationServiceUrl ;
                                                owl:cardinality "1"^^xsd:nonNegativeInteger
                                              ] ,
                                              [ rdf:type owl:Restriction ;
                                                owl:onProperty :hasFormula ;
                                                owl:qualifiedCardinality "1"^^xsd:nonNegativeInteger ;
                                                owl:onClass xsd:string
                                              ] ;
                              rdfs:comment "An indicator that can be computed by a service by providing a formular and variables." ;
                              rdfs:label "Simple computed value indicator" .


###  https://greeninfratwins.com/ns/grit#SpecifiedUseCase
:SpecifiedUseCase rdf:type owl:Class ;
                  rdfs:label "Specified use case" .


###  https://greeninfratwins.com/ns/grit#TechnicalQualityIndicator
:TechnicalQualityIndicator rdf:type owl:Class ;
                           rdfs:subClassOf :Indicator ;
                           rdfs:comment "An indicator for depicting the technical quality of a measure." ;
                           rdfs:label "Technical quality indicator" .


###  https://greeninfratwins.com/ns/grit#ValueIndicator
:ValueIndicator rdf:type owl:Class ;
                rdfs:subClassOf :Indicator ,
                                [ rdf:type owl:Restriction ;
                                  owl:onProperty :hasUnit ;
                                  owl:qualifiedCardinality "1"^^xsd:nonNegativeInteger ;
                                  owl:onClass <https://qudt.org/schema/qudt/Unit>
                                ] ,
                                [ rdf:type owl:Restriction ;
                                  owl:onProperty :hasValue ;
                                  owl:cardinality "1"^^xsd:nonNegativeInteger
                                ] ;
                rdfs:comment "A class for all value indicators and subclasses. Cannot be used for calculating. For constant values see \"git:ConstantValueIndicator\"." ;
                rdfs:label "Value indicator" ;
                rdfs:seeAlso :ConstantValueIndicator .


###  https://qudt.org/schema/qudt/Unit
<https://qudt.org/schema/qudt/Unit> rdf:type owl:Class .


###  https://schema.org/Person
<https://schema.org/Person> rdf:type owl:Class .


#################################################################
#    Individuals
#################################################################

###  https://greeninfratwins.com/ns/grit#Awf_1
:Awf_1 rdf:type owl:NamedIndividual ,
                :SpecifiedUseCase ;
       rdfs:label "Awf 1" .


###  https://greeninfratwins.com/ns/grit#Awf_2
:Awf_2 rdf:type owl:NamedIndividual ,
                :SpecifiedUseCase ;
       rdfs:label "Awf 2" .


###  https://greeninfratwins.com/ns/grit#Awf_3
:Awf_3 rdf:type owl:NamedIndividual ,
                :SpecifiedUseCase ;
       rdfs:label "Awf 3" .


###  https://greeninfratwins.com/ns/grit#Awf_4
:Awf_4 rdf:type owl:NamedIndividual ,
                :SpecifiedUseCase ;
       rdfs:label "Awf 4" .


###  https://greeninfratwins.com/ns/grit#IndicatorSet_Predefined_Availability
:IndicatorSet_Predefined_Availability rdf:type owl:NamedIndividual ,
                                               :IndicatorSet ;
                                      rdfs:label "Verfügbarkeit" .


###  https://greeninfratwins.com/ns/grit#IndicatorSet_Predefined_BuildingRelatedLifecycleCosts
:IndicatorSet_Predefined_BuildingRelatedLifecycleCosts rdf:type owl:NamedIndividual ,
                                                                :IndicatorSet ;
                                                       rdfs:label "Bauwerksbezogene Lebenszykluskosten" .


###  https://greeninfratwins.com/ns/grit#IndicatorSet_Predefined_CircularEconomyResources
:IndicatorSet_Predefined_CircularEconomyResources rdf:type owl:NamedIndividual ,
                                                           :IndicatorSet ;
                                                  rdfs:label "Kreislaufwirtschaft / Ressourcen" .


###  https://greeninfratwins.com/ns/grit#IndicatorSet_Predefined_EcologicalQuality
:IndicatorSet_Predefined_EcologicalQuality rdf:type owl:NamedIndividual ,
                                                    :IndicatorSet ;
                                           rdfs:label "Ökologische Qualität" .


###  https://greeninfratwins.com/ns/grit#IndicatorSet_Predefined_EconomicQuality
:IndicatorSet_Predefined_EconomicQuality rdf:type owl:NamedIndividual ,
                                                  :IndicatorSet ;
                                         rdfs:label "Ökonomische Qualität" .


###  https://greeninfratwins.com/ns/grit#IndicatorSet_Predefined_EnvironmentalEffects
:IndicatorSet_Predefined_EnvironmentalEffects rdf:type owl:NamedIndividual ,
                                                       :IndicatorSet ;
                                              rdfs:label "Externe Umwelteffekte" .


###  https://greeninfratwins.com/ns/grit#IndicatorSet_Predefined_ExternalCosts
:IndicatorSet_Predefined_ExternalCosts rdf:type owl:NamedIndividual ,
                                                :IndicatorSet ;
                                       rdfs:label "Externe Kosten (monetarisierte externe Effekte)" .


###  https://greeninfratwins.com/ns/grit#IndicatorSet_Predefined_HumanProtection
:IndicatorSet_Predefined_HumanProtection rdf:type owl:NamedIndividual ,
                                                  :IndicatorSet ;
                                         rdfs:label "Schutzgut Mensch" .


###  https://greeninfratwins.com/ns/grit#IndicatorSet_Predefined_LandUse
:IndicatorSet_Predefined_LandUse rdf:type owl:NamedIndividual ,
                                          :IndicatorSet ;
                                 rdfs:label "Flächeninanspruchnahme" .


###  https://greeninfratwins.com/ns/grit#IndicatorSet_Predefined_LifecycleAsessment
:IndicatorSet_Predefined_LifecycleAsessment rdf:type owl:NamedIndividual ,
                                                     :IndicatorSet ;
                                            rdfs:label "Ökobilanz" .


###  https://greeninfratwins.com/ns/grit#IndicatorSet_Predefined_LocalEnvironmentalRisks
:IndicatorSet_Predefined_LocalEnvironmentalRisks rdf:type owl:NamedIndividual ,
                                                          :IndicatorSet ;
                                                 rdfs:label "Risiken für die lokale Umwelt" .


###  https://greeninfratwins.com/ns/grit#IndicatorSet_Predefined_Reliability
:IndicatorSet_Predefined_Reliability rdf:type owl:NamedIndividual ,
                                              :IndicatorSet ;
                                     rdfs:label "Zuverlässigkeit" .


###  https://greeninfratwins.com/ns/grit#IndicatorSet_Predefined_Safety
:IndicatorSet_Predefined_Safety rdf:type owl:NamedIndividual ,
                                         :IndicatorSet ;
                                rdfs:label "Nutzersicherheit" .


###  https://greeninfratwins.com/ns/grit#IndicatorSet_Predefined_SocioCulturalQuality
:IndicatorSet_Predefined_SocioCulturalQuality rdf:type owl:NamedIndividual ,
                                                       :IndicatorSet ;
                                              rdfs:label "Sozio-kulturelle und funktionale Qualität" .


###  https://greeninfratwins.com/ns/grit#IndicatorSet_Predefined_TechnicalQuality
:IndicatorSet_Predefined_TechnicalQuality rdf:type owl:NamedIndividual ,
                                                   :IndicatorSet ;
                                          rdfs:label "Technische Qualität" .


###  https://greeninfratwins.com/ns/grit#IndicatorType_1_1_1
:IndicatorType_1_1_1 rdf:type owl:NamedIndividual ,
                              :IndicatorType ;
                     :hasIndicatorID "1.1.1" ;
                     rdfs:comment "Indikator für Definition von Materialität eines Bauwerks in Masse-Prozent" ;
                     rdfs:label "Materialität des Bauwerks" ;
                     :belongsToPredefinedSetOfIndicators :IndicatorSet_Predefined_CircularEconomyResources ,
                                                         :IndicatorSet_Predefined_EcologicalQuality .


###  https://greeninfratwins.com/ns/grit#IndicatorType_1_1_2
:IndicatorType_1_1_2 rdf:type owl:NamedIndividual ,
                              :IndicatorType ;
                     :hasIndicatorID "1.1.2" ;
                     rdfs:comment "Indikator für Definition von monetärer Materialwert in EUR" ;
                     rdfs:label "Monetärer Materialwert" ;
                     :belongsToPredefinedSetOfIndicators :IndicatorSet_Predefined_CircularEconomyResources ,
                                                         :IndicatorSet_Predefined_EcologicalQuality .


###  https://greeninfratwins.com/ns/grit#IndicatorType_1_1_3
:IndicatorType_1_1_3 rdf:type owl:NamedIndividual ,
                              :IndicatorType ;
                     :hasIndicatorID "1.1.3" ;
                     rdfs:comment "Indikator für Definition von Schad- und Risikostoffe in kg" ;
                     rdfs:label "Schad- und Risikostoffe" ;
                     :belongsToPredefinedSetOfIndicators :IndicatorSet_Predefined_CircularEconomyResources ,
                                                         :IndicatorSet_Predefined_EcologicalQuality .


###  https://greeninfratwins.com/ns/grit#IndicatorType_1_1_4
:IndicatorType_1_1_4 rdf:type owl:NamedIndividual ,
                              :IndicatorType ;
                     :hasIndicatorID "1.1.4" ;
                     rdfs:comment "Indikator für Definition von Demontagefaehigkeit mit qualitative Bewertungsergebnis" ;
                     rdfs:label "Demontagefähigkeit" ;
                     :belongsToPredefinedSetOfIndicators :IndicatorSet_Predefined_CircularEconomyResources ,
                                                         :IndicatorSet_Predefined_EcologicalQuality .


###  https://greeninfratwins.com/ns/grit#IndicatorType_1_1_5
:IndicatorType_1_1_5 rdf:type owl:NamedIndividual ,
                              :IndicatorType ;
                     :hasIndicatorID "1.1.5" ;
                     rdfs:comment "Indikator für Definition von Materialverwertung zur potentialen Kreislauffaehigkeit in Massen-Prozent" ;
                     rdfs:label "Materlaverwertung - Potentiale Kreislauffähigkeit" ;
                     :belongsToPredefinedSetOfIndicators :IndicatorSet_Predefined_CircularEconomyResources ,
                                                         :IndicatorSet_Predefined_EcologicalQuality .


###  https://greeninfratwins.com/ns/grit#IndicatorType_1_2_1
:IndicatorType_1_2_1 rdf:type owl:NamedIndividual ,
                              :IndicatorType ;
                     :hasIndicatorID "1.2.1" ;
                     rdfs:comment "Indikator für Definition Fläche des ökologisch gestörten Lebensraums durch Lärmbeeinträchtigung der Fauna in m2" ;
                     rdfs:label "Fläche des ökologisch gestörten Lebensraums durch Lärmbeeinträchtigung der Fauna" ;
                     :belongsToPredefinedSetOfIndicators :IndicatorSet_Predefined_EcologicalQuality ,
                                                         :IndicatorSet_Predefined_LocalEnvironmentalRisks .


###  https://greeninfratwins.com/ns/grit#IndicatorType_1_3_1
:IndicatorType_1_3_1 rdf:type owl:NamedIndividual ,
                              :IndicatorType ;
                     :hasIndicatorID "1.3.1" ;
                     rdfs:comment "Indikator für Definition von Flächeninanspruchnahme Bauwerk (dauerhaft) und Bauprozesse (vorübergehend) in gewichtete m2" ;
                     rdfs:label "Flächeninanspruchnahme (gesamt)" ;
                     :belongsToPredefinedSetOfIndicators :IndicatorSet_Predefined_EcologicalQuality ,
                                                         :IndicatorSet_Predefined_LandUse .


###  https://greeninfratwins.com/ns/grit#IndicatorType_1_3_1_1
:IndicatorType_1_3_1_1 rdf:type owl:NamedIndividual ,
                                :IndicatorType ;
                       :hasIndicatorID "1.3.1.1" ;
                       rdfs:comment "Indikator für Definition von Flächeninanspruchnahme Bauwerk (dauerhaft)  in gewichtete m2" ;
                       rdfs:label "Flächeninanspruchnahme Bauwerk (dauerhaft)" ;
                       :belongsToPredefinedSetOfIndicators :IndicatorSet_Predefined_EcologicalQuality ,
                                                           :IndicatorSet_Predefined_LandUse .


###  https://greeninfratwins.com/ns/grit#IndicatorType_1_3_1_2
:IndicatorType_1_3_1_2 rdf:type owl:NamedIndividual ,
                                :IndicatorType ;
                       :hasIndicatorID "1.3.1.2" ;
                       rdfs:comment "Indikator für Definition von Flächeninanspruchnahme Bauprozesse (vorübergehend) in gewichtete m2" ;
                       rdfs:label "Flächeninanspruchnahme Bauprozesse (vorübergehend)" ;
                       :belongsToPredefinedSetOfIndicators :IndicatorSet_Predefined_EcologicalQuality ,
                                                           :IndicatorSet_Predefined_LandUse .


###  https://greeninfratwins.com/ns/grit#IndicatorType_1_4_1
:IndicatorType_1_4_1 rdf:type owl:NamedIndividual ,
                              :IndicatorType ;
                     :hasIndicatorID "1.4.1" ;
                     rdfs:comment "Indikator für Definition von Verkehrsbedingte Emissionen infolge betrieblicher und baubedingter Verkehrsbeeinträchtigungen in Masse" ;
                     rdfs:label "Verkehrsbedingte Emissionen infolge betrieblicher und baubedingter Verkehrsbeeinträchtigungen (gesamt)" ;
                     :belongsToPredefinedSetOfIndicators :IndicatorSet_Predefined_EcologicalQuality ,
                                                         :IndicatorSet_Predefined_EnvironmentalEffects .


###  https://greeninfratwins.com/ns/grit#IndicatorType_1_4_1_1
:IndicatorType_1_4_1_1 rdf:type owl:NamedIndividual ,
                                :IndicatorType ;
                       :hasIndicatorID "1.4.1.1" ;
                       rdfs:comment "Indikator für Definition von Verkehrsbedingte Emissionen infolge betrieblicher und baubedingter Verkehrsbeeinträchtigungen in Masse" ;
                       rdfs:label "Verkehrsbedingte Emissionen infolge betrieblicher und baubedingter Verkehrsbeeinträchtigungen (CO2)" ;
                       :belongsToPredefinedSetOfIndicators :IndicatorSet_Predefined_EcologicalQuality ,
                                                           :IndicatorSet_Predefined_EnvironmentalEffects .


###  https://greeninfratwins.com/ns/grit#IndicatorType_1_4_1_2
:IndicatorType_1_4_1_2 rdf:type owl:NamedIndividual ,
                                :IndicatorType ;
                       :hasIndicatorID "1.4.1.2" ;
                       rdfs:comment "Indikator für Definition von Verkehrsbedingte Emissionen infolge betrieblicher und baubedingter Verkehrsbeeinträchtigungen in Masse" ;
                       rdfs:label "Verkehrsbedingte Emissionen infolge betrieblicher und baubedingter Verkehrsbeeinträchtigungen (NOx)" ;
                       :belongsToPredefinedSetOfIndicators :IndicatorSet_Predefined_EcologicalQuality ,
                                                           :IndicatorSet_Predefined_EnvironmentalEffects .


###  https://greeninfratwins.com/ns/grit#IndicatorType_1_4_1_3
:IndicatorType_1_4_1_3 rdf:type owl:NamedIndividual ,
                                :IndicatorType ;
                       :hasIndicatorID "1.4.1.3" ;
                       rdfs:comment "Indikator für Definition von Verkehrsbedingte Emissionen infolge betrieblicher und baubedingter Verkehrsbeeinträchtigungen in Masse" ;
                       rdfs:label "Verkehrsbedingte Emissionen infolge betrieblicher und baubedingter Verkehrsbeeinträchtigungen (PM2.5)" ;
                       :belongsToPredefinedSetOfIndicators :IndicatorSet_Predefined_EcologicalQuality ,
                                                           :IndicatorSet_Predefined_EnvironmentalEffects .


###  https://greeninfratwins.com/ns/grit#IndicatorType_1_4_1_4
:IndicatorType_1_4_1_4 rdf:type owl:NamedIndividual ,
                                :IndicatorType ;
                       :hasIndicatorID "1.4.1.4" ;
                       rdfs:comment "Indikator für Definition von Verkehrsbedingte Emissionen infolge betrieblicher und baubedingter Verkehrsbeeinträchtigungen in Masse" ;
                       rdfs:label "Verkehrsbedingte Emissionen infolge betrieblicher und baubedingter Verkehrsbeeinträchtigungen (PM5)" ;
                       :belongsToPredefinedSetOfIndicators :IndicatorSet_Predefined_EcologicalQuality ,
                                                           :IndicatorSet_Predefined_EnvironmentalEffects .


###  https://greeninfratwins.com/ns/grit#IndicatorType_1_4_1_5
:IndicatorType_1_4_1_5 rdf:type owl:NamedIndividual ,
                                :IndicatorType ;
                       :hasIndicatorID "1.4.1.5" ;
                       rdfs:comment "Indikator für Definition von Verkehrsbedingte Emissionen infolge betrieblicher und baubedingter Verkehrsbeeinträchtigungen in Masse" ;
                       rdfs:label "Verkehrsbedingte Emissionen infolge betrieblicher und baubedingter Verkehrsbeeinträchtigungen (PM10)" ;
                       :belongsToPredefinedSetOfIndicators :IndicatorSet_Predefined_EcologicalQuality ,
                                                           :IndicatorSet_Predefined_EnvironmentalEffects .


###  https://greeninfratwins.com/ns/grit#IndicatorType_1_5_1
:IndicatorType_1_5_1 rdf:type owl:NamedIndividual ,
                              :IndicatorType ;
                     :hasIndicatorID "1.5.1" ;
                     rdfs:comment "Indikator für Definition von Globales Erwärmungspotential (GWP) in kg CO2-Äquiv." ;
                     rdfs:label "Globales Erwärmungspotential (GWP)" ;
                     :belongsToPredefinedSetOfIndicators :IndicatorSet_Predefined_EcologicalQuality ,
                                                         :IndicatorSet_Predefined_LifecycleAsessment .


###  https://greeninfratwins.com/ns/grit#IndicatorType_1_5_2
:IndicatorType_1_5_2 rdf:type owl:NamedIndividual ,
                              :IndicatorType ;
                     :hasIndicatorID "1.5.2" ;
                     rdfs:comment "Indikator für Definition von Eutrophierungspotential (EP) in kg PO43-Äquiv." ;
                     rdfs:label "Eutrophierungspotential (EP)" ;
                     :belongsToPredefinedSetOfIndicators :IndicatorSet_Predefined_EcologicalQuality ,
                                                         :IndicatorSet_Predefined_LifecycleAsessment .


###  https://greeninfratwins.com/ns/grit#IndicatorType_1_5_3
:IndicatorType_1_5_3 rdf:type owl:NamedIndividual ,
                              :IndicatorType ;
                     :hasIndicatorID "1.5.3" ;
                     rdfs:comment "Indikator für Definition von Ozonschichtabbaupotential (ODP) in kg R11-Äquiv." ;
                     rdfs:label "Ozonschichtabbaupotential (ODP)" ;
                     :belongsToPredefinedSetOfIndicators :IndicatorSet_Predefined_EcologicalQuality ,
                                                         :IndicatorSet_Predefined_LifecycleAsessment .


###  https://greeninfratwins.com/ns/grit#IndicatorType_1_5_4
:IndicatorType_1_5_4 rdf:type owl:NamedIndividual ,
                              :IndicatorType ;
                     :hasIndicatorID "1.5.4" ;
                     rdfs:comment "Indikator für Definition von Versauerungspotential (AP) in kg SO2-Äquiv." ;
                     rdfs:label "Versauerungspotential (AP)" ;
                     :belongsToPredefinedSetOfIndicators :IndicatorSet_Predefined_EcologicalQuality ,
                                                         :IndicatorSet_Predefined_LifecycleAsessment .


###  https://greeninfratwins.com/ns/grit#IndicatorType_1_5_5
:IndicatorType_1_5_5 rdf:type owl:NamedIndividual ,
                              :IndicatorType ;
                     :hasIndicatorID "1.5.5" ;
                     rdfs:comment "Indikator für Definition von Ozonbildungspotential (POCP) in kg C2H4-Äquiv." ;
                     rdfs:label "Ozonbildungspotential (POCP)" ;
                     :belongsToPredefinedSetOfIndicators :IndicatorSet_Predefined_EcologicalQuality ,
                                                         :IndicatorSet_Predefined_LifecycleAsessment .


###  https://greeninfratwins.com/ns/grit#IndicatorType_1_5_6
:IndicatorType_1_5_6 rdf:type owl:NamedIndividual ,
                              :IndicatorType ;
                     :hasIndicatorID "1.5.6" ;
                     rdfs:comment "Indikator für Definition von Kumulierter Energieaufwand (KEA) in MJ" ;
                     rdfs:label "Kumulierter Energieaufwand (KEA)" ;
                     :belongsToPredefinedSetOfIndicators :IndicatorSet_Predefined_EcologicalQuality ,
                                                         :IndicatorSet_Predefined_LifecycleAsessment .


###  https://greeninfratwins.com/ns/grit#IndicatorType_2_1_1
:IndicatorType_2_1_1 rdf:type owl:NamedIndividual ,
                              :IndicatorType ;
                     :hasIndicatorID "2.1.1" ;
                     rdfs:comment "Indikator für Definition von Materialkosten, prozessbezogene Kosten (Planungs-, Baukosten, Kosten Nutzungsphase etc.) in EUR" ;
                     rdfs:label "Bauwerksbezogene Kosten" ;
                     :belongsToPredefinedSetOfIndicators :IndicatorSet_Predefined_BuildingRelatedLifecycleCosts ,
                                                         :IndicatorSet_Predefined_EconomicQuality .


###  https://greeninfratwins.com/ns/grit#IndicatorType_2_1_1_1
:IndicatorType_2_1_1_1 rdf:type owl:NamedIndividual ,
                                :IndicatorType ;
                       :hasIndicatorID "2.1.1.1" ;
                       rdfs:comment "Indikator für Definition von Materialkosten - Teilkosten von Material-, prozessbezogene Kosten (Planungs-, Baukosten, Kosten Nutzungsphase etc.) in EUR" ;
                       rdfs:label "Materialkosten" ;
                       :belongsToPredefinedSetOfIndicators :IndicatorSet_Predefined_BuildingRelatedLifecycleCosts ,
                                                           :IndicatorSet_Predefined_EconomicQuality .


###  https://greeninfratwins.com/ns/grit#IndicatorType_2_1_1_2
:IndicatorType_2_1_1_2 rdf:type owl:NamedIndividual ,
                                :IndicatorType ;
                       :hasIndicatorID "2.1.1.2" ;
                       rdfs:comment "Indikator für Definition von Prozessbezogenekosten, Teilkosten von Material-, prozessbezogene Kosten (Planungs-, Baukosten, Kosten Nutzungsphase etc.) in EUR" ;
                       rdfs:label "Prozessbezogene Kosten (Planungs-, Baukosten, Kosten Nutzungsphase etc.)" ;
                       :belongsToPredefinedSetOfIndicators :IndicatorSet_Predefined_BuildingRelatedLifecycleCosts ,
                                                           :IndicatorSet_Predefined_EconomicQuality .


###  https://greeninfratwins.com/ns/grit#IndicatorType_2_2_1
:IndicatorType_2_2_1 rdf:type owl:NamedIndividual ,
                              :IndicatorType ;
                     :hasIndicatorID "2.2.1" ;
                     rdfs:comment "Indikator für Definition von Kosten aufgrund von Zeitverlusten, Umleitungen und erhöhten Fahrzeugbetriebskosten in EUR" ;
                     rdfs:label "Kosten aufgrund von Zeitverlusten, Umleitungen und erhöhten Fahrzeugbetriebskosten " ;
                     :belongsToPredefinedSetOfIndicators :IndicatorSet_Predefined_EconomicQuality ,
                                                         :IndicatorSet_Predefined_ExternalCosts .


###  https://greeninfratwins.com/ns/grit#IndicatorType_3_1_1
:IndicatorType_3_1_1 rdf:type owl:NamedIndividual ,
                              :IndicatorType ;
                     :hasIndicatorID "3.1.1" ;
                     rdfs:comment "Indikator für Definition von Lärmbeeinträchtigung von Menschen (Laermpegel / Anzahl vom Lärm betroffene Personen)" ;
                     rdfs:label "Lärmbeeinträchtigung von Menschen (gesamt)" ;
                     :belongsToPredefinedSetOfIndicators :IndicatorSet_Predefined_HumanProtection ,
                                                         :IndicatorSet_Predefined_SocioCulturalQuality .


###  https://greeninfratwins.com/ns/grit#IndicatorType_3_1_1_1
:IndicatorType_3_1_1_1 rdf:type owl:NamedIndividual ,
                                :IndicatorType ;
                       :hasIndicatorID "3.1.1.1" ;
                       rdfs:comment "Indikator für Definition von Lärmbeeinträchtigung von Menschen (Lärmpegel / Anzahl vom Lärm betroffene Personen) in db/pax" ;
                       rdfs:label "Lärmbeeinträchtigung von Menschen (Lärmpegel / Anzahl vom Lärm betroffene Personen)" ;
                       :belongsToPredefinedSetOfIndicators :IndicatorSet_Predefined_HumanProtection ,
                                                           :IndicatorSet_Predefined_SocioCulturalQuality .


###  https://greeninfratwins.com/ns/grit#IndicatorType_3_1_1_2
:IndicatorType_3_1_1_2 rdf:type owl:NamedIndividual ,
                                :IndicatorType ;
                       :hasIndicatorID "3.1.1.2" ;
                       rdfs:comment "Indikator für Definition von Lärmbeeinträchtigung von Menschen (Anzahl vom Lärm betroffene Personen) in Konzentration Schadstoffe" ;
                       rdfs:label "Lärmbeeinträchtigung von Menschen (Anzahl vom Lärm betroffene Personen)" ;
                       :belongsToPredefinedSetOfIndicators :IndicatorSet_Predefined_HumanProtection ,
                                                           :IndicatorSet_Predefined_SocioCulturalQuality .


###  https://greeninfratwins.com/ns/grit#IndicatorType_3_1_3
:IndicatorType_3_1_3 rdf:type owl:NamedIndividual ,
                              :IndicatorType ;
                     :hasIndicatorID "3.1.3" ;
                     rdfs:comment "Indikator für Definition von Arbeitssicherheit (Anzahl an Unfällen / Unfallrate im Baustellenbereich) in pax / -" ;
                     rdfs:label "Arbeitssicherheit (Anzahl an Unfällen / Unfallrate im Baustellenbereich)" ;
                     :belongsToPredefinedSetOfIndicators :IndicatorSet_Predefined_HumanProtection ,
                                                         :IndicatorSet_Predefined_SocioCulturalQuality .


###  https://greeninfratwins.com/ns/grit#IndicatorType_3_2_1
:IndicatorType_3_2_1 rdf:type owl:NamedIndividual ,
                              :IndicatorType ;
                     :hasIndicatorID "3.2.1" ;
                     rdfs:comment "Indikator für Definition von Reduktion der zeitbezogenen Kapazität (Zeitverluste der Reisezeit; Veränderung Zuverlässigkeit der Reisezeit) in %" ;
                     rdfs:label "Reduktion der zeitbezogenen Kapazität (Zeitverluste der Reisezeit; Veränderung Zuverlässigkeit der Reisezeit)" ;
                     :belongsToPredefinedSetOfIndicators :IndicatorSet_Predefined_Availability ,
                                                         :IndicatorSet_Predefined_SocioCulturalQuality .


###  https://greeninfratwins.com/ns/grit#IndicatorType_4_1_1
:IndicatorType_4_1_1 rdf:type owl:NamedIndividual ,
                              :IndicatorType ;
                     :hasIndicatorID "4.1.1" ;
                     rdfs:comment "Indikator für Definition von Zuverlässigkeitsindex (β-Wert)" ;
                     rdfs:label "Zuverlässigkeitsindex (β-Wert)" ;
                     :belongsToPredefinedSetOfIndicators :IndicatorSet_Predefined_Reliability ,
                                                         :IndicatorSet_Predefined_TechnicalQuality .


###  https://greeninfratwins.com/ns/grit#IndicatorType_4_2_1
:IndicatorType_4_2_1 rdf:type owl:NamedIndividual ,
                              :IndicatorType ;
                     :hasIndicatorID "4.2.1" ;
                     rdfs:comment "Indikator für Definition von Anzahl an Unfällen/Unfallrate im Normalbetrieb (bezogen auf den Zustand)" ;
                     rdfs:label "Anzahl an Unfällen/Unfallrate im Normalbetrieb (bezogen auf den Zustand)" ;
                     :belongsToPredefinedSetOfIndicators :IndicatorSet_Predefined_Safety ,
                                                         :IndicatorSet_Predefined_TechnicalQuality .


#################################################################
#    Annotations
#################################################################

:hasIfcGuid rdfs:label "has ifc guid" .


###  Generated by the OWL API (version 5.1.18) https://github.com/owlcs/owlapi/
